coq/theories/ITree/Guarded.v
@@ -1,0 +1,170 @@
+From Coinduction Require Import coinduction tactics.
+
+From OGS Require Import Prelude.
+From OGS.Utils Require Import Rel.
+From OGS.Game Require Import Event.
+From OGS.ITree Require Import ITree Structure Eq.
+
+Module stuff.
+  Context {I} {E : event I I}.
+
+  Definition eqn R X Y : Type := X ⇒ᵢ itree E (Y +ᵢ R) .
+  Definition apply_eqn {R X Y} (q : eqn R X Y) : itree E (X +ᵢ R) ⇒ᵢ itree E (Y +ᵢ R) :=
+    fun _ t => t >>= fun _ r => match r with
+                            | inl x => q _ x
+                            | inr y => Ret' (inr y)
+                            end .
+
+  Variant guarded' {X Y i} : itree' E (X +ᵢ Y) i -> Type :=
+  | GRet y : guarded' (RetF (inr y))
+  | GTau t : guarded' (TauF t)
+  | GVis e k : guarded' (VisF e k)
+  .
+  Definition guarded {X Y i} (t : itree E (X +ᵢ Y) i) := guarded' t.(_observe). 
+  Definition eqn_guarded {R X Y} (e : eqn R X Y) : Type := forall i (x : X i), guarded (e i x) .
+
+  Definition apply_guarded_l {R X Y} (e : eqn R X Y) {i} (t : itree E (X +ᵢ R) i)
+             : guarded t -> guarded (apply_eqn e _ t) .
+  intro H; unfold guarded in *; cbn in *.
+  destruct t.(_observe); dependent elimination H; cbn; econstructor.
+  Defined.
+
+  Definition apply_guarded_r {R X Y} (e : eqn R X Y) (H : eqn_guarded e) {i} (t : itree E (X +ᵢ R) i)
+             : guarded (apply_eqn e _ t) .
+    unfold guarded in *; cbn in *.
+    destruct (_observe t) as [ [] | | ]; try econstructor.
+    exact (H _ x).
+  Defined.
+  
+  Definition iter_guarded_aux {R X} (e : eqn R X X) (H : eqn_guarded e) : itree E (X +ᵢ R) ⇒ᵢ itree E R :=
+    cofix CIH i t := go match t.(_observe) with
+                        | RetF (inl x) => match H i x with
+                                          | GRet y => RetF y
+                                          | GTau t => TauF (CIH _ t)
+                                          | GVis e k => VisF e (fun r => CIH _ (k r))
+                                          end
+                        | RetF (inr y) => RetF y
+                        | TauF t => TauF (CIH _ t)
+                        | VisF e k => VisF e (fun r => CIH _ (k r))
+                        end .
+
+  Definition iter_guarded {R X} (e : eqn R X X) (H : eqn_guarded e) : X ⇒ᵢ itree E R :=
+    fun _ x => iter_guarded_aux e H _ (e _ x) .
+
+  Lemma iter_guarded_unfold {X Y RY} {_ : Reflexiveᵢ RY} (f : eqn Y X X) (H : eqn_guarded f) {i x}
+    : it_eq RY
+        (iter_guarded f H i x)
+        (bind (f i x) (fun _ r => match r with
+                                | inl x => iter_guarded f H _ x
+                                | inr y => Ret' y end)).
+    unfold iter_guarded; remember (f i x) as t; clear Heqt; clear x.
+    revert i t; unfold it_eq; coinduction R CIH; intros i t.
+    cbn; pose (ot := _observe t); fold ot; destruct ot as [ [] | | ]; cbn; auto.
+    pose (Hix := H i x); pose (fix_ := f i x); fold Hix; fold fix_ in Hix |- *.
+    destruct (Hix); auto.
+  Qed.
+
+  (*
+  Lemma iter_guarded_lem {X Y RY} {_ : Equivalenceᵢ RY} (f : eqn Y X X) (g : X ⇒ᵢ itree E Y)
+                 (H0 : eqn_guarded f)
+                 (H : forall i x, it_eq RY (g i x) (bind (f i x) (fun _ r => match r with
+                                                  | inl x => g _ x
+                                                  | inr y => Ret' y end)))
+                 : forall i x, it_eq RY (g i x) (iter_guarded f H0 i x).
+    unfold it_eq; coinduction R CIH; intros i x.
+    etransitivity; [ | symmetry; apply it_eq_t_bt, (iter_guarded_unfold f H0) ].
+    rewrite (H i x); cbn.
+    pose (a := (f i x).(_observe)); fold a.
+    pose (Ha := H0 i x); unfold guarded in Ha; fold a in Ha.
+    destruct Ha; cbn; econstructor; auto; [ | intro r ].
+    all: change (subst ?f _ ?t) with (bind t f).
+    all: eapply (tt_t (it_eq_map E RY)).
+    all: refine (it_eq_up2bind_t _ _ _ _ _ _ _); econstructor; eauto.
+    all: intros ? ? ? <-; destruct x1; auto.
+  Qed.
+*)
+
+  (* eventually guarded equations *)
+
+  Inductive ev_guarded' {X Y} (e : eqn Y X X) {i} : itree' E (X +ᵢ Y) i -> Type :=
+  | GHead t : guarded' t -> ev_guarded' e t
+  | GNext x : ev_guarded' e (e i x).(_observe) -> ev_guarded' e (RetF (inl x))
+  .
+  #[global] Arguments GHead {X Y e i}.
+  #[global] Arguments GNext {X Y e i}.
+
+  Definition ev_guarded {X Y} (e : eqn Y X X) {i} (t : itree E (X +ᵢ Y) i) := ev_guarded' e t.(_observe).
+  Definition eqn_ev_guarded {X Y} (e : eqn Y X X) : Type := forall i (x : X i), ev_guarded e (e i x) .
+  
+  Equations evg_unroll {X Y} (e : eqn Y X X) {i} (t : itree' E (X +ᵢ Y) i) (p : ev_guarded' e t)
+    : itree E (X +ᵢ Y) i :=
+    evg_unroll e t (GHead _ g) := go t ;
+    evg_unroll e t (GNext x p) := apply_eqn e _ (evg_unroll e (e i x).(_observe) p) .
+
+  Equations evg_unroll_guarded {X Y} (e : eqn Y X X) {i} (t : itree' E (X +ᵢ Y) i) (p : ev_guarded' e t)
+    : guarded (evg_unroll e t p) :=
+    evg_unroll_guarded e t (GHead _ g) := g ;
+    evg_unroll_guarded e t (GNext x p) := apply_guarded_l e _ (evg_unroll_guarded e _ p) . 
+
+  Definition eqn_evg_unroll {X Y} (e : eqn Y X X) (H : eqn_ev_guarded e) : eqn Y X X
+    := fun _ x => evg_unroll e (e _ x).(_observe) (H _ x) .
+
+  Definition eqn_evg_unroll_guarded {X Y} (e : eqn Y X X) (H : eqn_ev_guarded e)
+    : eqn_guarded (eqn_evg_unroll e H)
+    := fun _ x => evg_unroll_guarded e (e _ x).(_observe) (H _ x) .
+
+  Definition iter_ev_guarded {R X} (e : eqn R X X) (H : eqn_ev_guarded e) : X ⇒ᵢ itree E R :=
+    iter_guarded _ (eqn_evg_unroll_guarded e H) .
+
+  Lemma iter_evg_unfold_aux {X Y RY} {_ : Reflexiveᵢ RY} (f : eqn Y X X) (H : eqn_ev_guarded f) {i}
+                  (t : itree E (X +ᵢ Y) i)
+                  
+    : it_eq RY
+        (iter_guarded_aux (eqn_evg_unroll f H) (eqn_evg_unroll_guarded f H) i t)
+        (t >>= fun (i0 : I) (r : (X +ᵢ Y) i0) =>
+             match r with
+             | inl x => iter_guarded (eqn_evg_unroll f H) (eqn_evg_unroll_guarded f H) i0 x
+             | inr y => Ret' y
+             end) .
+    revert i t; unfold it_eq; coinduction R CIH; intros i t.
+    cbn; destruct (_observe t) as [ [] | | ]; try econstructor; auto.
+    clear t; cbn; unfold eqn_evg_unroll_guarded at 1, eqn_evg_unroll at 3.
+    remember (H i x) as q; unfold ev_guarded in q.
+    pose (u := (f i x).(_observe)); fold u in q |- *.
+    clear Heqq; remember u as z ; clear Heqz u.
+    induction q; cbn.
+    * destruct g; auto.
+    * unfold apply_guarded_l.
+      pose (z := _observe (f i x0)).
+      fold z in q ,IHq |- *; remember z as z'; clear Heqz' z.
+      pose (tg := evg_unroll_guarded f z' q); fold tg in IHq |- *; unfold guarded in tg.
+      destruct tg; cbn; auto.
+  Qed.
+
+  Lemma iter_evg_unfold {X Y RY} {_ : Reflexiveᵢ RY} (f : eqn Y X X) (H : eqn_ev_guarded f) {i x}
+    : it_eq RY
+        (iter_ev_guarded f H i x)
+        (bind (f i x) (fun _ r => match r with
+                                | inl x => iter_ev_guarded f H _ x
+                                | inr y => Ret' y end)).
+    unfold iter_ev_guarded at 1, iter_guarded, eqn_evg_unroll at 2.
+    pose (t' := f i x); change (f i x >>= ?a) with (t' >>= a).
+    remember t' as t; unfold t' in Heqt; clear t'.
+    (* AHHHHHHHHHH
+    revert Heqt; induction (H i x); intro Heqt; cbn
+    - now apply it_eq_unstep.
+    unfold eqn_evg_unroll at 1.
+    pose (u := f i x).
+    remember (H i x) as p. fold u in p.
+    change (it_eqF E RY (it_eq RY) i _ _)
+      with (it_eqF E RY (it_eq RY) i
+              (_observe (iter_guarded_aux (eqn_evg_unroll f H) (eqn_evg_unroll_guarded f H) i (evg_unroll f (_observe u) p)))
+              (_observe (bind (go (_observe u)) (fun _ r => match r with
+                                          | inl x => iter_guarded (eqn_evg_unroll f H)
+                                                      (eqn_evg_unroll_guarded f H) _ x
+                                          | inr y => Ret' y end)))).
+    *)
+    Admitted.
+
+
+End stuff.
