coq/theories/ITree/Properties.v
@@ -1,0 +1,231 @@
+From Coinduction Require Import coinduction tactics.
+
+From OGS Require Import Prelude.
+From OGS.Utils Require Import Rel.
+From OGS.Game Require Import Event.
+From OGS.ITree Require Import ITree Structure Eq.
+
+Module stuff.
+  Context {I} {E : event I I}.
+  
+  #[global] Instance fmap_eq {X RX Y RY} {f : X ⇒ᵢ Y} {_ : forall i, Proper (@RX i ==> @RY i) (f i)} {i}
+            : Proper (it_eq RX (i:=i) ==> it_eq RY (i:=i)) (fmap (E:=E) f i).
+  Proof.
+    unfold Proper, respectful, it_eq.
+    revert i; coinduction R CIH; intros i x y h.
+    apply (gfp_fp (it_eq_map E RX)) in h.
+    cbn in *; cbv [observe] in h; dependent destruction h; simpl_depind; eauto.
+    econstructor; now apply H.
+  Qed.
+
+  #[global] Instance subst_eq {X Y} {RX : relᵢ X X} {RY : relᵢ Y Y}
+    : Proper (dpointwise_relation (fun i => RX i ==> it_eq RY (i:=i))
+              ==> dpointwise_relation (fun i => it_eq RX (i:=i) ==> it_eq RY (i:=i)))
+        (@subst I E X Y).
+  Proof.
+    unfold Proper, respectful, dpointwise_relation, pointwise_relation, it_eq.
+    intros f g h1; coinduction R CIH; intros i x y h2.
+    apply (gfp_fp (it_eq_map E RX)) in h2.
+    cbn in *; cbv [observe] in h2; dependent destruction h2; simpl_depind; eauto.
+    pose (h3 := h1 i _ _ r_rel).
+    apply (gfp_fp (it_eq_map E RY)) in h3.
+    cbn in h3; cbv [observe] in h3.
+    dependent destruction h3; simpl_depind; econstructor; eauto.
+    2: intro.
+    all: now apply (gfp_t (it_eq_map E RY)).
+  Qed.
+  
+  #[global] Instance subst_eat {X Y} (f : X ⇒ᵢ itree E Y) {i}
+   : Proper (it_eat' i ==> it_eat' i) (subst f i).
+  Proof.
+    intros ? ? H; unfold it_eat' in *; cbn.
+    remember (_observe x) as _x eqn:Hx; clear Hx.
+    remember (_observe y) as _y eqn:Hy; clear Hy.
+    dependent induction H; now econstructor.
+  Qed.    
+
+  Lemma bind_bind_com {X Y Z RZ} {_ : Reflexiveᵢ RZ} {f : X ⇒ᵢ itree E Y} {g : Y ⇒ᵢ itree E Z} {i} {x : itree E X i}
+    : it_eq RZ (bind (bind x f) g) (bind x (kcomp f g)).
+  Proof.
+    revert i x; unfold it_eq; coinduction R CIH; intros i x.
+    cbn; destruct (x.(_observe)); eauto.
+    destruct ((f i r).(_observe)); eauto.
+    destruct ((g i r0).(_observe)); eauto.
+  Qed.
+
+  Lemma fmap_bind_com {X Y Z RZ} {_ : Reflexiveᵢ RZ} {f : X ⇒ᵢ Y} {g : Y ⇒ᵢ itree E Z} {i} {x : itree E X i}
+    : it_eq RZ (bind (fmap f _ x) g) (bind x (fun i x => g i (f i x))).
+  Proof.
+    revert i x; unfold it_eq; coinduction R CIH; intros i x.
+    cbn; destruct (x.(_observe)); eauto.
+    destruct ((g i (f i r)).(_observe)); eauto.
+  Qed.
+
+  Lemma bind_fmap_com {X Y Z RZ} {_ : Reflexiveᵢ RZ} {f : X ⇒ᵢ itree E Y} {g : Y ⇒ᵢ Z} {i} {x : itree E X i}
+    : it_eq RZ (fmap g _ (bind x f)) (bind x (fun i x => fmap g i (f i x))).
+  Proof.
+    revert i x; unfold it_eq; coinduction R CIH; intros i x.
+    cbn; destruct (x.(_observe)); eauto.
+    destruct ((f i r).(_observe)); eauto.
+  Qed.
+
+  Lemma subst_subst {X Y Z} (f : Y ⇒ᵢ itree E Z) (g : X ⇒ᵢ itree E Y) {i} (x : itree E X i)
+      : ((x >>= g) >>= f) ≊ (x >>= (g >=> f)) .
+  Proof. apply bind_bind_com. Qed.
+
+  Variant bindR {X1 X2 Y1 Y2} (RX : relᵢ X1 X2) (R : relᵢ (itree E X1) (itree E X2))
+                (S : relᵢ (itree E Y1) (itree E Y2))
+          : relᵢ (itree E Y1) (itree E Y2) :=
+    | BindR {i t1 t2 k1 k2}
+        (u : R i t1 t2)
+        (v : forall i x1 x2, RX i x1 x2 -> S i (k1 i x1) (k2 i x2))
+      : bindR RX R S i (t1 >>= k1) (t2 >>= k2).
+  Arguments BindR {X1 X2 Y1 Y2 RX R S i t1 t2 k1 k2}.    
+  #[global] Hint Constructors bindR : core.
+
+  Program Definition bindR_eq_map {X1 X2 Y1 Y2} (RX : relᵢ X1 X2) : mon (relᵢ (itree E Y1) (itree E Y2)) :=
+    {| body S := bindR RX (@it_eq _ E _ _ RX) S ;
+       Hbody _ _ H _ _ _ '(BindR u v) := BindR u (fun i _ _ r => H _ _ _ (v i _ _ r)) |}.
+
+  Lemma it_eq_up2bind_t {X1 X2 Y1 Y2} RX RY : @bindR_eq_map X1 X2 Y1 Y2 RX <= it_eq_t E RY.
+  Proof.
+    apply Coinduction; intros R i x y [ ? ? ? ? ? u v].
+    unfold it_eq in u; apply (gfp_fp (it_eq_map E RX)) in u.
+    cbn in *; cbv [observe] in u.
+    dependent destruction u; simpl_depind.
+    - refine (it_eqF_mon _ _ (id_T _ _ R) _ _ _ (v i0 _ _ r_rel)).
+    - econstructor; apply (fTf_Tf (it_eq_map E RY)).
+      refine (BindR t_rel (fun i _ _ r => b_T (it_eq_map E RY) _ _ _ _ _ (v i _ _ r))).
+    - econstructor; intros r; apply (fTf_Tf (it_eq_map E RY)).
+      refine (BindR (k_rel r) (fun i _ _ r => b_T (it_eq_map E RY) _ _ _ _ _ (v i _ _ r))).
+  Qed.
+
+  Program Definition bindR_w_map {X1 X2 Y1 Y2} (RX : relᵢ X1 X2) : mon (relᵢ (itree E Y1) (itree E Y2)) :=
+    {| body S := bindR RX (@it_wbisim _ E _ _ RX) S ;
+       Hbody _ _ H _ _ _ '(BindR u v) := BindR u (fun i _ _ r => H _ _ _ (v i _ _ r)) |}.
+
+  Lemma it_wbisim_up2bind_t {X1 X2 Y1 Y2} RX RY : @bindR_w_map X1 X2 Y1 Y2 RX <= it_wbisim_t E RY.
+  Proof.
+    apply Coinduction; intros R i x y [ ? ? ? ? ? u v].
+    unfold it_wbisim in u; apply (gfp_fp (it_wbisim_map E RX)) in u.
+    cbn in *; cbv [observe] in u.
+    destruct u as [? ? r1 r2 rr]; dependent destruction rr.
+    - destruct (v _ _ _ r_rel) as [ ? ? s1 s2 ss]; econstructor.
+      etransitivity; [ exact (subst_eat _ _ (Ret' _) r1) | exact s1 ].
+      etransitivity; [ exact (subst_eat _ _ (Ret' _) r2) | exact s2 ].
+      now apply (it_eqF_mon _ _ (id_T _ _ R)).
+   - econstructor.
+     exact (subst_eat _ _ (Tau' _) r1).
+     exact (subst_eat _ _ (Tau' _) r2).
+     cbn; econstructor.
+     apply (fTf_Tf (it_wbisim_map E RY)).
+     econstructor; [ apply t_rel | intros; now apply (b_T (it_wbisim_map E RY)), v ].
+   - econstructor.
+     exact (subst_eat _ _ (Vis' _ _) r1).
+     exact (subst_eat _ _ (Vis' _ _) r2).
+     cbn; econstructor; intro r.
+     apply (fTf_Tf (it_wbisim_map E RY)).
+     econstructor; [ apply k_rel | intros; now apply (b_T (it_wbisim_map E RY)), v ].
+ Qed.
+
+  Lemma iter_cong_strong {X1 X2 Y1 Y2} {RX : relᵢ X1 X2} {RY : relᵢ Y1 Y2}
+                      f g (_ : forall i a b, RX i a b ->  it_eq (sumᵣ RX RY) (f i a) (g i b))
+                      : forall i a b, RX i a b -> it_eq (E:=E) RY (iter f i a) (iter g i b).
+  Proof.
+    unfold it_eq; coinduction R CIH; intros i a b r.
+    pose (h1 := H i a b r).
+    apply it_eq_step in h1; cbn in *; cbv [observe] in h1.
+    dependent destruction h1; simpl_depind.
+    - destruct r_rel; eauto.
+    - econstructor.
+      apply (tt_t (it_eq_map E _)); cbn.
+      apply (it_eq_up2bind_t (sumᵣ RX RY) RY); econstructor; eauto.
+      intros ? ? ? []; apply (tt_t (it_eq_map E RY)), (b_t (it_eq_map E RY)); cbn; eauto.
+    - econstructor; intro.
+      apply (tt_t (it_eq_map E _)); cbn.
+      apply (it_eq_up2bind_t (sumᵣ RX RY) RY); econstructor; eauto.
+      intros ? ? ? []; apply (bt_t (it_eq_map E RY)); cbn; eauto.
+  Qed.
+
+  #[global] Instance iter_proper_strong {X Y} {RX : relᵢ X X} {RY : relᵢ Y Y}
+    : Proper (dpointwise_relation (fun i => RX i ==> it_eq (sumᵣ RX RY) (i:=i))
+              ==> dpointwise_relation (fun i => RX i ==> it_eq RY (i:=i)))
+        (@iter I E X Y)
+    := iter_cong_strong.
+
+  Lemma iter_cong_weak {X1 X2 Y1 Y2} {RX : relᵢ X1 X2} {RY : relᵢ Y1 Y2}
+                      f g (_ : forall i a b, RX i a b -> it_wbisim (sumᵣ RX RY) i (f i a) (g i b))
+                      : forall i a b, RX i a b -> it_wbisim (E:=E) RY i (iter f i a) (iter g i b).
+  Proof.
+    unfold it_wbisim; coinduction R CIH; intros i a b r.
+    pose (H1 := H i a b r).
+    apply it_wbisim_step in H1.
+    cbn in *; cbv [observe] in H1.
+    destruct H1 as [ ? ? r1 r2 rr ]; dependent destruction rr.
+    - destruct r_rel.
+      * pose (H2 := H _ _ _ H0).
+        apply it_wbisim_step in H2.
+        destruct H2 as [ ? ? s1 s2 ss ].
+        econstructor.
+        exact (subst_eat _ _ (Ret' _) r1).
+        exact (subst_eat _ _ (Ret' _) r2).
+        cbn; econstructor.
+        now apply CIH.
+      * econstructor.
+        exact (subst_eat _ _ (Ret' _) r1).
+        exact (subst_eat _ _ (Ret' _) r2).
+        now cbn; econstructor.
+    - econstructor.
+      exact (subst_eat _ _ (Tau' _) r1).
+      exact (subst_eat _ _ (Tau' _) r2).
+      cbn; econstructor.
+      apply (tt_t (it_wbisim_map E _)); cbn.
+      apply (it_wbisim_up2bind_t (sumᵣ RX RY) RY); econstructor; eauto.
+      intros ? ? ? []; apply (tt_t (it_wbisim_map E RY)), (b_t (it_wbisim_map E RY)); cbn; eauto.
+    - econstructor.
+      exact (subst_eat _ _ (Vis' _ _) r1).
+      exact (subst_eat _ _ (Vis' _ _) r2).
+      cbn; econstructor; intro.
+      apply (tt_t (it_wbisim_map E _)); cbn.
+      apply (it_wbisim_up2bind_t (sumᵣ RX RY) RY); econstructor; [ apply k_rel | ].
+      intros ? ? ? []; apply (tt_t (it_wbisim_map E RY)), (b_t (it_wbisim_map E RY)); cbn; eauto.
+  Qed.
+
+  #[global] Instance iter_weq {X Y} {RX : relᵢ X X} {RY : relᵢ Y Y}
+    : Proper (dpointwise_relation (fun i => RX i ==> it_wbisim (sumᵣ RX RY) i)
+              ==> dpointwise_relation (fun i => RX i ==> it_wbisim RY i))
+        (@iter I E X Y)
+    := iter_cong_weak.
+
+  Lemma iter_unfold {X Y RY} {_ : Reflexiveᵢ RY} (f : X ⇒ᵢ itree E (X +ᵢ Y)) {i x}
+    : it_eq RY
+        (iter f i x)
+        (bind (f i x) (fun _ r => go (match r with
+                                   | inl x => TauF (iter f _ x)
+                                   | inr y => RetF y end))).
+  Proof.
+    apply (gfp_fp (it_eq_map E RY)).
+    cbn; destruct (_observe (f i x)); auto.
+    destruct r; eauto.
+  Qed.
+  
+  Lemma iter_lem {X Y RY} {_ : Equivalenceᵢ RY} (f : X ⇒ᵢ itree E (X +ᵢ Y)) (g : X ⇒ᵢ itree E Y)
+                 (H : forall i x, it_eq RY (g i x) (bind (f i x) (fun _ r => go (match r with
+                                                  | inl x => TauF (g _ x)
+                                                  | inr y => RetF y end))))
+                 : forall i x, it_eq RY (g i x) (iter f i x).
+  Proof.
+    unfold it_eq; coinduction R CIH; intros i x.
+    apply (bt_tbt (it_eq_map E RY)).
+    etransitivity.
+    now unshelve eapply (Hbody (it_eq_t E RY) _ _ _ _ _ _ (H i x)).
+    etransitivity; cycle 1.
+    symmetry; now unshelve eapply (Hbody (it_eq_t E RY) _ _ _ _ _ _ (iter_unfold f)).
+    eapply (it_eq_up2bind_t (eqᵢ (X +ᵢ Y)) RY).
+    econstructor. reflexivity.
+    intros ? ? [] ->; econstructor.
+    now apply CIH.
+    reflexivity.
+  Qed.
+
+End stuff.
