coq/theories/ITree/Structure.v
@@ -1,0 +1,57 @@
+From OGS Require Import Prelude.
+From OGS.Game Require Import Event.
+From OGS.ITree Require Import ITree.
+
+Section monad.
+  Context {I} {E : event I I}.
+
+  Definition eat_one_tau {X i} (t : itree E X i) : itree E X i :=
+    go match t.(_observe) with
+       | RetF x => RetF x
+       | TauF t => t.(_observe)
+       | VisF q k => VisF q k
+       end .
+
+  Definition fmap {X Y} (f : X ⇒ᵢ Y) : itree E X ⇒ᵢ itree E Y :=
+    cofix _fmap _ u :=
+      go match u.(_observe) with
+         | RetF r => RetF (f _ r)
+         | TauF t => TauF (_fmap _ t)
+         | VisF e k => VisF e (fun r => _fmap _ (k r))
+         end.
+
+  Definition subst {X Y} (f : X ⇒ᵢ itree E Y) : itree E X ⇒ᵢ itree E Y :=
+    cofix _subst _ u :=
+      go match u.(_observe) with
+         | RetF r => (f _ r).(_observe)
+         | TauF t => TauF (_subst _ t)
+         | VisF e k => VisF e (fun r => _subst _ (k r))
+         end.
+
+  Definition bind {X Y i} x f := @subst X Y f i x.
+
+  Definition kcomp {X Y Z} (f : X ⇒ᵢ itree E Y) (g : Y ⇒ᵢ itree E Z) : X ⇒ᵢ itree E Z :=
+    fun i x => bind (f i x) g.
+
+  Definition iter {X Y} (f : X ⇒ᵢ itree E (X +ᵢ Y)) : X ⇒ᵢ itree E Y :=
+    cofix _iter _ x :=
+      bind (f _ x) (fun _ r => go match r with
+                                | inl x => TauF (_iter _ x)
+                                | inr y => RetF y
+                                end) .
+
+End monad.
+
+#[global] Notation "f <$> x" := (fmap f x) (at level 30).
+#[global] Notation "x >>= f" := (bind x f) (at level 30).
+#[global] Notation "f =<< x" := (subst f _ x) (at level 30).
+#[global] Notation "f >=> g" := (kcomp f g) (at level 30).
+
+Definition emap {I} {A B : event I I} (F : A ⇒ₑ B) {X} : itree A X ⇒ᵢ itree B X :=
+  cofix _emap _ u :=
+      go match u.(_observe) with
+         | RetF r => RetF r
+         | TauF t => TauF (_emap _ t)
+         | VisF e k => VisF (F.(ea_qry) e)
+                           (fun r => _emap _ (rew (F.(ea_nxt)) in k (F.(ea_rsp) r)))
+         end.
